agda/univalence.agda
@@ -1,146 +1,72 @@
 {-# OPTIONS --without-K --exact-split --safe #-}
 
 {-
-  univalence definitions
+  univalence
 -}
 
 open import Agda.Primitive
 open import logic
-open import types
 open import path
-open import hlevel
-open import retract
-
-{-
-  Voevodsky's equivalence
--}
-
--- space: witnesses x' × f x' = y
-fiber : {X :  Set ℓ} {Y : Set ℓ₁} (f : X → Y) → Y → Set (ℓ ⊔ ℓ₁)
-fiber {ℓ}{ℓ₁} {X}{Y} f y = Σ x ∶ X , f x ＝ y
-
-fiber-base : {X : Set ℓ} {Y : Set ℓ₁} {f : X → Y} {y : Y}
-           → fiber f y → X
-fiber-base (x , p) = x
-
-fiber-id : {X : Set ℓ} {Y : Set ℓ₁} {f : X → Y} {y : Y}
-         → (w : fiber f y) → f (fiber-base w) ＝ y
-fiber-id (x , p) = p
-
--- the fibre (preimage) of all y : Y under f is unique (size 1)
--- the proof is also unique, via the characterisation of Σ identity
-is-equiv : {X : Set ℓ} {Y : Set ℓ₁} → (X → Y) → Set (ℓ ⊔ ℓ₁)
-is-equiv {ℓ}{ℓ₁} {X}{Y} f = Π y ∶ Y , is-contr (fiber f y)
+open import equiv
 
 _≃_ : Set ℓ₁ → Set ℓ₂ → Set (ℓ₁ ⊔ ℓ₂)
-X ≃ Y = Σ f ∶ (X → Y) , is-equiv f
+X ≃ Y = Σ f ∶ (X → Y) , is-equivalence f
 infix 5 _≃_
 
 equiv-fn : {X : Set ℓ} {Y : Set ℓ₁} → X ≃ Y → X → Y
 equiv-fn (f , i) = f
 
-id-is-equiv : (X : Set ℓ) → is-equiv id
-id-is-equiv = singleton-types-are-singletons
+equiv-proof : {X : Set ℓ} {Y : Set ℓ₁} → X ≃ Y → X → Y
+equiv-proof (f , i) = f
 
 refl≃ : (X : Set ℓ) → X ≃ X
-refl≃ X = id , id-is-equiv X
+refl≃ X = id , id-is-equivalence X
 
--- inverses - center is p , Σ x, f x ＝ y
-inverse : {X : Set ℓ} {Y : Set ℓ₁} (f : X → Y) → is-equiv f → (Y → X)
-inverse f equiv y = fiber-base (center (fiber f y) (equiv y))
+_●_ : {X : Set ℓ} {Y : Set ℓ₁} {Z : Set ℓ₂} → X ≃ Y → Y ≃ Z → X ≃ Z
+(f , d) ● (f' , e) = f' ∘ f , equivalence-∘ e d
+trans≃ = _●_
+
+sym≃ : {X : Set ℓ} {Y : Set ℓ₁} → X ≃ Y → Y ≃ X
+sym≃ (f , e) = inverse f e , inverse-is-equivalence e
+
+_≃⟨_⟩_ : (X : Set ℓ) {Y : Set ℓ₁} {Z : Set ℓ₂} → X ≃ Y → Y ≃ Z → X ≃ Z
+_ ≃⟨ d ⟩ e = d ● e
+infixr 2 _≃⟨_⟩_
+
+_■ : (X : Set ℓ) → X ≃ X
+_■ = refl≃
+infix 3 _■
+
+idtoeq : (X Y : Set ℓ) → X ＝ Y → X ≃ Y
+idtoeq X X (refl X) = refl≃ X
 
 {-
-  relationship with invertibles
+  ua is the other direction
 -}
 
-invertible : {A : Set ℓ} {B : Set ℓ₁} (f : A → B) → Set (ℓ ⊔ ℓ₁)
-invertible {ℓ}{ℓ₁} {A}{B} f = Σ g ∶ (B → A) , g ∘ f ~ id × f ∘ g ~ id
+is-univalent : (ℓ : Level) → Set (lsuc ℓ)
+is-univalent ℓ = ∀ (X Y : Set ℓ) → is-equivalence (idtoeq X Y)
 
--- the easy direction
-inverses-are-sections : {X : Set ℓ} {Y : Set ℓ₁} (f : X → Y) (e : is-equiv f)
-                      → f ∘ inverse f e ~ id
-inverses-are-sections f e y = fiber-id (center (fiber f y) (e y))
+univalence-≃ : is-univalent ℓ → (X Y : Set ℓ) → (X ＝ Y) ≃ (X ≃ Y)
+univalence-≃ univalence X Y = idtoeq X Y , univalence X Y
 
-inverse-centrality : {X : Set ℓ} {Y : Set ℓ₁}
-                     (f : X → Y) (e : is-equiv f) (y : Y) (t : fiber f y)
-                   → (inverse f e y , inverses-are-sections f e y) ＝ t
-inverse-centrality f e y = centrality (fiber f y) (e y)
+ua : is-univalent ℓ → (X Y : Set ℓ) → X ≃ Y → X ＝ Y
+ua univalence X Y = inverse (idtoeq X Y) (univalence X Y)
 
-inverses-are-retractions : {X : Set ℓ} {Y : Set ℓ₁} (f : X → Y) (e : is-equiv f)
-                         → inverse f e ∘ f ~ id
-inverses-are-retractions f e x = ap pr₁ r
-  where
-    q : ∀ fb → (center _ (e (f x))) ＝ fb
-    q = centrality _ (e (f x))
-    -- inverse is just the base of the single fiber
-    r : center (fiber f (f x)) (e (f x)) ＝ (x , refl (f x))
-    r = q (x , refl (f x))
-
-equivs-are-invertible : {X : Set ℓ} {Y : Set ℓ₁} (f : X → Y)
-                      → is-equiv f → invertible f
-equivs-are-invertible f e = inverse f e ,
-                            inverses-are-retractions f e ,
-                            inverses-are-sections f e
-
--- the hard direction
-rap : {X : Set ℓ} {Y : Set ℓ₁} {x y : X} (f : X → Y)
-    → has-retraction f → (f x ＝ f y) → (x ＝ y)
-rap {ℓ}{ℓ₁}{X}{Y} {x}{y} f (g , gf) p = sym＝ (gf x) ∙ (ap g p) ∙ gf y
-
-ap-rap : {X : Set ℓ} {Y : Set ℓ₁} {x y : X}
-       → (f : X → Y) (r : has-retraction f)
-       → (p : x ＝ y) → rap f r (ap f p) ＝ p
-ap-rap {ℓ}{ℓ₁}{X}{Y} {x}{y} f (g , gf) (refl x)
-  = ap (λ e → sym＝ (gf x) ∙ e) (sym＝ (p＝refl∙p (gf x))) ∙ iv∙p＝refl _
-
-invertibles-are-equivs : {X : Set ℓ} {Y : Set ℓ₁} (f : X → Y)
-                       → invertible f → is-equiv f
-invertibles-are-equivs {ℓ}{ℓ₁} {X}{Y} f (g , gf , fg) y₀ = proof
-  where
-    -- to show (Σ x ∶ X , f x ＝ y₀) ◁ (Σ x ∶ X , g (f x) ＝ g y₀)
-    test : (x : X) → (f x ＝ y₀) ◁ (g (f x) ＝ g y₀)
-    test x = rap g (f , fg) , ap g , ap-rap g (f , fg)
-
-    hom-iso : ∀ x → (g (f x) ＝ g y₀) ◁ (x ＝ g y₀)
-    hom-iso x = transport (λ - → - ＝ g y₀) (sym＝ (gf x)) ,
-                transport (_＝ g y₀) (gf x) ,
-                transport-is-section (_＝ g y₀) (gf x)
-
-    -- want to show the fiber type is a retract of a singleton(-type)
-    fiber-is-singleton-Σ-retract : (fiber f y₀) ◁ (Σ x ∶ X , x ＝ g y₀)
-    fiber-is-singleton-Σ-retract
-      = (Σ x ∶ X , f x ＝ y₀)       ◁⟨ Σ-retract test ⟩
-        (Σ x ∶ X , g (f x) ＝ g y₀) ◁⟨ Σ-retract hom-iso ⟩
-        (Σ x ∶ X , x ＝ g y₀)       ◀ -- these are just ∙ (sym＝) gf which cancel
-
-    proof : Σ c ∶ (fiber f y₀) , is-center _ c
-    proof = retract-of-singleton fiber-is-singleton-Σ-retract
-              (singleton-types-are-singletons _ (g y₀))
-
-
--- corollaries
--- inverses-are-equivs : {X : Set ℓ} {Y : Set ℓ₁} (f : X → Y) (e : is-equiv f)
---                     → is-equiv (inverse f e)
--- inverses-are-equivs = {!!}
+ua-transport : {X Y : Set ℓ} → X ＝ Y → X → Y
+ua-transport {ℓ} {X} {Y} p = equiv-fn (idtoeq X Y p)
 
 {-
-  univalence
+  conversion
 -}
 
 quasi-equiv : (A : Set ℓ) (B : Set ℓ₁) → Set (ℓ ⊔ ℓ₁)
 quasi-equiv A B = Σ f ∶ (A → B) , invertible f
 
-Id→Eq : (X Y : Set ℓ) → X ＝ Y → X ≃ Y
-Id→Eq X X (refl X) = refl≃ X
+invertible-to-≃ : {X : Set ℓ} {Y : Set ℓ₁} (f : X → Y)
+                → invertible f → X ≃ Y
+invertible-to-≃ f i = f , invertibles-are-equivalences f i
 
-is-univalent : (ℓ : Level) → Set (lsuc ℓ)
-is-univalent ℓ = ∀ (X Y : Set ℓ) → is-equiv (Id→Eq X Y)
-
-univalence-≃ : is-univalent ℓ → (X Y : Set ℓ) → (X ＝ Y) ≃ (X ≃ Y)
-univalence-≃ ua X Y = Id→Eq X Y , ua X Y
-
-Eq→Id : is-univalent ℓ → (X Y : Set ℓ) → X ≃ Y → X ＝ Y
-Eq→Id ua X Y = inverse (Id→Eq X Y) (ua X Y)
-
-Id→fun : {X Y : Set ℓ} → X ＝ Y → X → Y
-Id→fun {ℓ} {X} {Y} p = equiv-fn (Id→Eq X Y p)
+{-
+  TODO examples
+-}
